src/GoCompilationLemmas.v
@@ -359,6 +359,14 @@ Proof.
     cancel.
 Qed.
 
+Lemma source_stmt_many_declares : forall decls cont,
+    (forall vars, source_stmt (cont vars)) ->
+    source_stmt (many_declares decls cont).
+Proof.
+  induction decls; eauto; intros.
+  destruct a; econstructor; eauto.
+Qed.
+
 Lemma CompileVar : forall env A var T (v : T) {H : GoWrapper T},
   EXTRACT Ret v
   {{ var ~> v * A }}
@@ -757,6 +765,7 @@ Proof.
   rewrite middle_split1.
   comp_apply CompileMiddle; divisibility.
 Qed.
+
 
 Lemma CompileIf : forall V varb (b : bool)
   (ptrue pfalse : prog V) xptrue xpfalse F G env,
@@ -1164,6 +1173,185 @@ Proof.
   repeat econstructor.
   all: eval_expr; [reflexivity].
 Qed.
+
+Definition middle_immut : forall low mid high w, immut_word mid := Rec.middle.
+
+Fixpoint go_rec_type (t : Rec.type) : type :=
+  match t with
+  | Rec.WordF n => ImmutableBuffer
+  | Rec.ArrayF t' n => Slice (go_rec_type t')
+  | Rec.RecF fs =>
+    (fix rec_type fs :=
+       match fs with
+       | [] => Struct []
+       | (_, f) :: fs' => Pair (go_rec_type f) (rec_type fs')
+       end) fs
+  end.
+
+Instance GoWrapper_rec t : GoWrapper (Rec.data t).
+  einduction t using Rec.type_rect_nest; simpl.
+  - change word with immut_word. typeclasses eauto.
+  - typeclasses eauto.
+  - apply IHt0.
+  - simpl; typeclasses eauto.
+  - simpl in *; typeclasses eauto.
+Defined.
+
+Lemma GoWrapper_rec_go_rec_type : forall t, @wrap_type _ (GoWrapper_rec t) = go_rec_type t.
+Proof.
+  einduction t using Rec.type_rect_nest; simpl; auto.
+  - rewrite <- IHt0; reflexivity.
+  - apply IHt0.
+  - reflexivity.
+  - simpl in *.
+    rewrite <- IHt0.
+    rewrite <- IHt1.
+    reflexivity.
+Qed.
+
+Fixpoint go_of_word (t : Rec.type) (vdst vsrc : var) (from : nat) : stmt :=
+  match t with
+  | Rec.WordF n =>
+    Declare Num (fun vfrom =>
+      Declare Num (fun vto =>
+        (Modify (@SetConst Num from) ^(vfrom); Modify (@SetConst Num (from + n)) ^(vto);
+         Modify SliceBuffer ^(vdst, vsrc, vfrom, vto))))
+  | Rec.ArrayF t' n =>
+    (fix array_of_word n from :=
+       match n with
+       | O => Modify (@SetConst (Slice (go_rec_type t')) (Here [])) ^(vdst)
+       | S n' =>
+         Declare (go_rec_type t') (fun vt' =>
+           (array_of_word n' from;
+            go_of_word t' vt' vsrc from;
+            Modify AppendOp ^(vdst, vt')))
+       end) n from
+  | Rec.RecF fs =>
+    (fix rec_of_word fs vdst from :=
+       match fs with
+       | [] => Modify (@SetConst (Struct []) tt) ^(vdst)
+       | (_, f) :: fs' =>
+         Declare (go_rec_type f) (fun vf =>
+           Declare (go_rec_type (Rec.RecF fs')) (fun vfs' =>
+             (go_of_word f vf vsrc from;
+              rec_of_word fs' vfs' (from + Rec.len f);
+              Modify JoinPair ^(vdst, vf, vfs')
+              )))
+       end) fs vdst from
+  end%go.
+
+Hint Constructors source_stmt. 
+Lemma source_stmt_go_of_word : forall t vsrc vdst from,
+    source_stmt (go_of_word t vdst vsrc from).
+Proof.
+  intros t vsrc.
+  induction t using Rec.type_rect_nest
+  with (Q := fun rt =>
+               forall vdst from, source_stmt ((fix rec_of_word fs vdst from :=
+       match fs with
+       | [] => Modify (@SetConst (Struct []) tt) ^(vdst)
+       | (_, f) :: fs' =>
+         Declare (go_rec_type f) (fun vf =>
+           Declare (go_rec_type (Rec.RecF fs')) (fun vfs' =>
+             (go_of_word f vf vsrc from;
+              rec_of_word fs' vfs' (from + Rec.len f);
+              Modify JoinPair ^(vdst, vf, vfs')
+              )))%go
+       end) rt vdst from)); simpl; intros.
+  - eauto.
+  - induction n; eauto.
+  - eapply IHt.
+  - eauto.
+  - eauto.
+Qed.
+
+Require Import PeanoNat.
+
+Fixpoint byte_aligned (t : Rec.type) : Prop :=
+  match t with
+  | Rec.WordF n => Nat.divide 8 n
+  | Rec.ArrayF t' n => byte_aligned t'
+  | Rec.RecF fs =>
+    (fix fields_aligned fs :=
+       match fs with
+       | [] => True
+       | (_, f) :: fs' =>
+         byte_aligned f /\ fields_aligned fs'
+       end) fs
+  end%go.
+
+Lemma compile_of_word' : forall (t : Rec.type) (vdst vsrc : var) before after (buf : immut_word (before + (Rec.len t + after))) env F,
+    byte_aligned t ->
+    Nat.divide 8 before ->
+    Nat.divide 8 after ->
+    EXTRACT Ret (@Rec.of_word_middle t before after buf)
+    {{ vdst ~>? Rec.data t * vsrc ~> buf * F }}
+      go_of_word t vdst vsrc before
+    {{ fun ret => vdst ~> ret * vsrc ~> buf * F }} // env.
+Proof.
+  einduction t using Rec.type_rect_nest; simpl; intros.
+  - pose proof (@CompileDeclare env (word n) nat _) as Hc.
+    eapply Hc; intros.
+    eapply Hc; intros.
+    eapply hoare_weaken.
+    eapply CompileBefore.
+    eapply hoare_weaken; [ let H' := fresh in pose proof (@CompileConst' nat _ env) as H'; eapply H' | cancel_go.. ].
+    2: cancel_go.
+    2: cancel_go.
+    eapply CompileBefore.
+    eapply hoare_weaken; [ let H' := fresh in pose proof (@CompileConst' nat _ env) as H'; eapply H' | cancel_go.. ].
+    fold plus.
+    eapply hoare_weaken; [ eapply CompileMiddle; eauto | cancel_go.. ].
+  - induction n; simpl.
+    + eapply hoare_weaken.
+      evar (F' : pred).
+      pose proof (@CompileConst (list (Rec.data t0)) _ env F' vdst []).
+      subst F'.
+      simpl in H2.
+      rewrite GoWrapper_rec_go_rec_type in H2.
+      apply H2.
+      rewrite GoWrapper_rec_go_rec_type. cancel_go.
+      cancel_go.
+    + eapply hoare_weaken. rewrite <- GoWrapper_rec_go_rec_type. eapply CompileDeclare; intros.
+    eapply extract_equiv_prog.
+    match goal with
+    | [ |- ProgMonad.prog_equiv _ ?pr ] =>
+      let Pr := fresh "Pr" in
+      set pr as Pr;
+      match goal with
+      | [ Pr := context[@Rec.of_word_middle ?a ?b ?c ?d] |- _ ] =>
+        pattern (@Rec.of_word_middle a b c d) in Pr
+      end
+    end.
+      subst Pr.
+      eapply bind_left_id.
+      eapply hoare_weaken.
+      eapply CompileBindRet.
+      eapply hoare_weaken.
+      rewrite GoWrapper_rec_go_rec_type.
+      eapply IHn.
+Admitted.
+
+Lemma compile_of_word : forall (t : Rec.type) (vdst vsrc : var) (buf : immut_word (Rec.len t)) env F,
+    byte_aligned t ->
+    EXTRACT Ret (@Rec.of_word t buf)
+    {{ vdst ~>? Rec.data t * vsrc ~> buf * F }}
+      go_of_word t vdst vsrc 0
+    {{ fun ret => vdst ~> ret * vsrc ~> buf * F }} // env.
+Proof.
+  intros.
+  erewrite Rec.of_word_middle_eq.
+  eapply hoare_weaken.
+  eapply compile_of_word'; try divisibility.
+  rewrite okToCancel_eq_rect_immut_word.
+  reflexivity.
+  intros; cbv beta.
+  rewrite okToCancel_eq_rect_immut_word.
+  reflexivity.
+  Unshelve.
+  eapply plus_n_O.
+Qed.
+
 
 Lemma CompileUncons :
   forall env T F G V {Wr: GoWrapper V} (lvar cvar xvar xsvar : var) (l : list V)
